zoo_std: mpsc_flag → flag_mpsc

theories/zoo_std/flag_mpsc.v
@@ -3,45 +3,45 @@ Require Import zoo.common.countable.
 Require Import zoo.iris.base_logic.lib.excl.
 Require Import zoo.iris.base_logic.lib.oneshot.
 Require Import zoo.base.
-Require Export zoo_std.mpsc_flag__code.
-Require Import zoo_std.mpsc_flag__types.
+Require Export zoo_std.flag_mpsc__code.
+Require Import zoo_std.flag_mpsc__types.
 Require Import zoo.options.
 
 Implicit Type b : bool.
 
-Class MpscFlagG Σ `{zoo۰G : !ZooG Σ} :=
-  { #[local] mpsc_flag۰G۰state۰G :: OneshotG Σ () ()
-  ; #[local] mpsc_flag۰G۰consumer۰G :: ExclG Σ unitO
+Class FlagMpscG Σ `{zoo۰G : !ZooG Σ} :=
+  { #[local] flag_mpsc۰G۰state۰G :: OneshotG Σ () ()
+  ; #[local] flag_mpsc۰G۰consumer۰G :: ExclG Σ unitO
   }.
 
-Definition mpsc_flag۰Σ :=
+Definition flag_mpsc۰Σ :=
   #[oneshot۰Σ () ()
   ; excl۰Σ unitO
   ].
-#[global] Instance subGｰmpsc_flag۰Σ `{zoo۰G : !ZooG Σ} :
-  subG mpsc_flag۰Σ Σ →
-  MpscFlagG Σ.
+#[global] Instance subGｰflag_mpsc۰Σ `{zoo۰G : !ZooG Σ} :
+  subG flag_mpsc۰Σ Σ →
+  FlagMpscG Σ.
 Proof.
   solve_inG.
 Qed.
 
 Module base.
-  Section mpsc_flag۰G.
-    Context `{mpsc_flag۰G : MpscFlagG Σ}.
+  Section flag_mpsc۰G.
+    Context `{flag_mpsc۰G : FlagMpscG Σ}.
 
     Implicit Type t : location.
     Implicit Type P : iProp Σ.
 
-    Record mpsc_flag۰name :=
-      { mpsc_flag۰name۰state : gname
-      ; mpsc_flag۰name۰consumer : gname
+    Record flag_mpsc۰name :=
+      { flag_mpsc۰name۰state : gname
+      ; flag_mpsc۰name۰consumer : gname
       }.
-    Implicit Type γ : mpsc_flag۰name.
+    Implicit Type γ : flag_mpsc۰name.
 
-    #[global] Instance mpsc_flag۰nameｰeq_dec : EqDecision mpsc_flag۰name :=
+    #[global] Instance flag_mpsc۰nameｰeq_dec : EqDecision flag_mpsc۰name :=
       ltac:(solve_decision).
-    #[global] Instance mpsc_flag۰nameｰcountable :
-      Countable mpsc_flag۰name.
+    #[global] Instance flag_mpsc۰nameｰcountable :
+      Countable flag_mpsc۰name.
     Proof.
       solve_countable.
     Qed.
@@ -49,16 +49,16 @@ Module base.
     #[local] Definition state۰unset' γ_state :=
       oneshot۰pending γ_state Own ().
     #[local] Definition state۰unset γ :=
-      state۰unset' γ.(mpsc_flag۰name۰state).
+      state۰unset' γ.(flag_mpsc۰name۰state).
     #[local] Definition state۰set' γ_state :=
       oneshot۰shot γ_state ().
     #[local] Definition state۰set γ :=
-      state۰set' γ.(mpsc_flag۰name۰state).
+      state۰set' γ.(flag_mpsc۰name۰state).
 
     #[local] Definition consumer' γ_consumer :=
       excl γ_consumer ().
     #[local] Definition consumer γ :=
-      consumer' γ.(mpsc_flag۰name۰consumer).
+      consumer' γ.(flag_mpsc۰name۰consumer).
 
     #[local] Definition inv۰consumer γ P : iProp Σ :=
       P ∨ consumer γ.
@@ -88,59 +88,59 @@ Module base.
         & Hb
         )
       ".
-    Definition mpsc_flag۰inv t γ P :=
+    Definition flag_mpsc۰inv t γ P :=
       inv nroot (inv۰inner t γ P).
     #[local] Instance : CustomIpat "inv" :=
       " #Hinv
       ".
 
-    Definition mpsc_flag۰consumer :=
+    Definition flag_mpsc۰consumer :=
       consumer.
     #[local] Instance : CustomIpat "consumer" :=
       " Hconsumer
       ".
 
-    Definition mpsc_flag۰resolved :=
+    Definition flag_mpsc۰resolved :=
       state۰set.
     #[local] Instance : CustomIpat "resolved" :=
       " #Hstate_set
       ".
 
-    #[global] Instance mpsc_flag۰invｰcontractive t γ :
-      Contractive (mpsc_flag۰inv t γ).
+    #[global] Instance flag_mpsc۰invｰcontractive t γ :
+      Contractive (flag_mpsc۰inv t γ).
     Proof.
-      rewrite /mpsc_flag۰inv /inv۰inner /inv۰set  /inv۰consumer.
+      rewrite /flag_mpsc۰inv /inv۰inner /inv۰set  /inv۰consumer.
       solve_contractive.
     Qed.
-    #[global] Instance mpsc_flag۰invｰne t γ :
-      NonExpansive (mpsc_flag۰inv t γ).
+    #[global] Instance flag_mpsc۰invｰne t γ :
+      NonExpansive (flag_mpsc۰inv t γ).
     Proof.
       apply _.
     Qed.
-    #[global] Instance mpsc_flag۰invｰproper t γ :
-      Proper ((≡) ==> (≡)) (mpsc_flag۰inv t γ).
-    Proof.
-      apply _.
-    Qed.
-
-    #[global] Instance mpsc_flag۰consumerｰtimeless γ :
-      Timeless (mpsc_flag۰consumer γ).
-    Proof.
-      apply _.
-    Qed.
-    #[global] Instance mpsc_flag۰resolvedｰtimeless γ :
-      Timeless (mpsc_flag۰resolved γ).
+    #[global] Instance flag_mpsc۰invｰproper t γ :
+      Proper ((≡) ==> (≡)) (flag_mpsc۰inv t γ).
     Proof.
       apply _.
     Qed.
 
-    #[global] Instance mpsc_flag۰invｰpersistent t γ P :
-      Persistent (mpsc_flag۰inv t γ P).
+    #[global] Instance flag_mpsc۰consumerｰtimeless γ :
+      Timeless (flag_mpsc۰consumer γ).
     Proof.
       apply _.
     Qed.
-    #[global] Instance mpsc_flag۰resolvedｰpersistent γ :
-      Persistent (mpsc_flag۰resolved γ).
+    #[global] Instance flag_mpsc۰resolvedｰtimeless γ :
+      Timeless (flag_mpsc۰resolved γ).
+    Proof.
+      apply _.
+    Qed.
+
+    #[global] Instance flag_mpsc۰invｰpersistent t γ P :
+      Persistent (flag_mpsc۰inv t γ P).
+    Proof.
+      apply _.
+    Qed.
+    #[global] Instance flag_mpsc۰resolvedｰpersistent γ :
+      Persistent (flag_mpsc۰resolved γ).
     Proof.
       apply _.
     Qed.
@@ -181,25 +181,25 @@ Module base.
       apply exclｰexclusive.
     Qed.
 
-    Lemma mpsc_flag۰consumerｰexclusive γ :
-      mpsc_flag۰consumer γ -∗
-      mpsc_flag۰consumer γ -∗
+    Lemma flag_mpsc۰consumerｰexclusive γ :
+      flag_mpsc۰consumer γ -∗
+      flag_mpsc۰consumer γ -∗
       False.
     Proof.
       apply consumerｰexclusive.
     Qed.
 
-    Lemma mpsc_flag٠createｰspec P :
+    Lemma flag_mpsc٠createｰspec P :
       {{{
         True
       }}}
-        mpsc_flag٠create ()
+        flag_mpsc٠create ()
       {{{
         t γ
       , RET #t;
         meta_token t ⊤ ∗
-        mpsc_flag۰inv t γ P ∗
-        mpsc_flag۰consumer γ
+        flag_mpsc۰inv t γ P ∗
+        flag_mpsc۰consumer γ
       }}}.
     Proof.
       iIntros "%Φ _ HΦ".
@@ -211,27 +211,27 @@ Module base.
       iMod consumerｰalloc as "(%γ_consumer & Hconsumer)".
 
       pose γ :=
-        {|mpsc_flag۰name۰state := γ_state
-        ; mpsc_flag۰name۰consumer := γ_consumer
+        {|flag_mpsc۰name۰state := γ_state
+        ; flag_mpsc۰name۰consumer := γ_consumer
         |}.
 
       iApply ("HΦ" $! t γ).
       iFrameSteps.
     Qed.
 
-    Lemma mpsc_flag٠getｰspec t γ P :
+    Lemma flag_mpsc٠getｰspec t γ P :
       {{{
-        mpsc_flag۰inv t γ P ∗
-        mpsc_flag۰consumer γ
+        flag_mpsc۰inv t γ P ∗
+        flag_mpsc۰consumer γ
       }}}
-        mpsc_flag٠get #t
+        flag_mpsc٠get #t
       {{{
         b
       , RET #b;
         if b then
           P
         else
-          mpsc_flag۰consumer γ
+          flag_mpsc۰consumer γ
       }}}.
     Proof.
       iIntros "%Φ ((:inv) & (:consumer)) HΦ".
@@ -250,15 +250,15 @@ Module base.
       - iFrameSteps.
     Qed.
 
-    Lemma mpsc_flag٠setｰspec t γ P :
+    Lemma flag_mpsc٠setｰspec t γ P :
       {{{
-        mpsc_flag۰inv t γ P ∗
+        flag_mpsc۰inv t γ P ∗
         ▷ P
       }}}
-        mpsc_flag٠set #t
+        flag_mpsc٠set #t
       {{{
         RET ();
-        mpsc_flag۰resolved γ
+        flag_mpsc۰resolved γ
       }}}.
     Proof.
       iIntros "%Φ ((:inv) & HP) HΦ".
@@ -271,27 +271,27 @@ Module base.
       iMod (stateｰupdate with "Hb") as "#Hstate_set".
       iFrameSteps.
     Qed.
-  End mpsc_flag۰G.
+  End flag_mpsc۰G.
 
-  #[global] Opaque mpsc_flag۰inv.
-  #[global] Opaque mpsc_flag۰consumer.
-  #[global] Opaque mpsc_flag۰resolved.
+  #[global] Opaque flag_mpsc۰inv.
+  #[global] Opaque flag_mpsc۰consumer.
+  #[global] Opaque flag_mpsc۰resolved.
 End base.
 
-Require zoo_std.mpsc_flag__opaque.
+Require zoo_std.flag_mpsc__opaque.
 
-Section mpsc_flag۰G.
-  Context `{mpsc_flag۰G : MpscFlagG Σ}.
+Section flag_mpsc۰G.
+  Context `{flag_mpsc۰G : FlagMpscG Σ}.
 
   Implicit Type 𝑡 : location.
   Implicit Type t : val.
   Implicit Type P : iProp Σ.
 
-  Definition mpsc_flag۰inv t P : iProp Σ :=
+  Definition flag_mpsc۰inv t P : iProp Σ :=
     ∃ 𝑡 γ,
     ⌜t = #𝑡⌝ ∗
     𝑡 ↪ γ ∗
-    base.mpsc_flag۰inv 𝑡 γ P.
+    base.flag_mpsc۰inv 𝑡 γ P.
   #[local] Instance : CustomIpat "inv" :=
     " ( %l{}
       & %γ{}
@@ -301,11 +301,11 @@ Section mpsc_flag۰G.
       )
     ".
 
-  Definition mpsc_flag۰consumer t : iProp Σ :=
+  Definition flag_mpsc۰consumer t : iProp Σ :=
     ∃ 𝑡 γ,
     ⌜t = #𝑡⌝ ∗
     𝑡 ↪ γ ∗
-    base.mpsc_flag۰consumer γ.
+    base.flag_mpsc۰consumer γ.
   #[local] Instance : CustomIpat "consumer" :=
     " ( %l{;_}
       & %γ{;_}
@@ -315,11 +315,11 @@ Section mpsc_flag۰G.
       )
     ".
 
-  Definition mpsc_flag۰resolved t : iProp Σ :=
+  Definition flag_mpsc۰resolved t : iProp Σ :=
     ∃ 𝑡 γ,
     ⌜t = #𝑡⌝ ∗
     𝑡 ↪ γ ∗
-    base.mpsc_flag۰resolved γ.
+    base.flag_mpsc۰resolved γ.
   #[local] Instance : CustomIpat "resolved" :=
     " ( %l{;_}
       & %γ{;_}
@@ -329,114 +329,114 @@ Section mpsc_flag۰G.
       )
     ".
 
-  #[global] Instance mpsc_flag۰invｰcontractive t :
-    Contractive (mpsc_flag۰inv t).
+  #[global] Instance flag_mpsc۰invｰcontractive t :
+    Contractive (flag_mpsc۰inv t).
   Proof.
     solve_contractive.
   Qed.
-  #[global] Instance mpsc_flag۰invｰne t :
-    NonExpansive (mpsc_flag۰inv t).
+  #[global] Instance flag_mpsc۰invｰne t :
+    NonExpansive (flag_mpsc۰inv t).
   Proof.
     apply _.
   Qed.
-  #[global] Instance mpsc_flag۰invｰproper t :
-    Proper ((≡) ==> (≡)) (mpsc_flag۰inv t).
-  Proof.
-    apply _.
-  Qed.
-
-  #[global] Instance mpsc_flag۰consumerｰtimeless t :
-    Timeless (mpsc_flag۰consumer t).
-  Proof.
-    apply _.
-  Qed.
-  #[global] Instance mpsc_flag۰resolvedｰtimeless t :
-    Timeless (mpsc_flag۰resolved t).
+  #[global] Instance flag_mpsc۰invｰproper t :
+    Proper ((≡) ==> (≡)) (flag_mpsc۰inv t).
   Proof.
     apply _.
   Qed.
 
-  #[global] Instance mpsc_flag۰invｰpersistent t P :
-    Persistent (mpsc_flag۰inv t P).
+  #[global] Instance flag_mpsc۰consumerｰtimeless t :
+    Timeless (flag_mpsc۰consumer t).
   Proof.
     apply _.
   Qed.
-  #[global] Instance mpsc_flag۰resolvedｰpersistent t :
-    Persistent (mpsc_flag۰resolved t).
+  #[global] Instance flag_mpsc۰resolvedｰtimeless t :
+    Timeless (flag_mpsc۰resolved t).
   Proof.
     apply _.
   Qed.
 
-  Lemma mpsc_flag۰consumerｰexclusive t :
-    mpsc_flag۰consumer t -∗
-    mpsc_flag۰consumer t -∗
+  #[global] Instance flag_mpsc۰invｰpersistent t P :
+    Persistent (flag_mpsc۰inv t P).
+  Proof.
+    apply _.
+  Qed.
+  #[global] Instance flag_mpsc۰resolvedｰpersistent t :
+    Persistent (flag_mpsc۰resolved t).
+  Proof.
+    apply _.
+  Qed.
+
+  Lemma flag_mpsc۰consumerｰexclusive t :
+    flag_mpsc۰consumer t -∗
+    flag_mpsc۰consumer t -∗
     False.
   Proof.
     iIntros "(:consumer =1) (:consumer =2)". simp.
     iDestruct (metaｰagree with "Hmeta_1 Hmeta_2") as %->.
-    iApply (base.mpsc_flag۰consumerｰexclusive with "Hconsumer_1 Hconsumer_2").
+    iApply (base.flag_mpsc۰consumerｰexclusive with "Hconsumer_1 Hconsumer_2").
   Qed.
 
-  Lemma mpsc_flag٠createｰspec P :
+  Lemma flag_mpsc٠createｰspec P :
     {{{
       True
     }}}
-      mpsc_flag٠create ()
+      flag_mpsc٠create ()
     {{{
       t
     , RET t;
-      mpsc_flag۰inv t P ∗
-      mpsc_flag۰consumer t
+      flag_mpsc۰inv t P ∗
+      flag_mpsc۰consumer t
     }}}.
   Proof.
     iIntros "%Φ _ HΦ".
 
     iApply wpｰfupd.
-    wp۰apply (base.mpsc_flag٠createｰspec with "[//]") as (𝑡 γ) "(Hmeta & Hinv & Hconsumer)".
+    wp۰apply (base.flag_mpsc٠createｰspec with "[//]") as (𝑡 γ) "(Hmeta & Hinv & Hconsumer)".
     iMod (metaｰset γ with "Hmeta") as "#Hmeta"; first done.
     iSteps.
   Qed.
 
-  Lemma mpsc_flag٠getｰspec t P :
+  Lemma flag_mpsc٠getｰspec t P :
     {{{
-      mpsc_flag۰inv t P ∗
-      mpsc_flag۰consumer t
+      flag_mpsc۰inv t P ∗
+      flag_mpsc۰consumer t
     }}}
-      mpsc_flag٠get t
+      flag_mpsc٠get t
     {{{
       b
     , RET #b;
       if b then
         P
       else
-        mpsc_flag۰consumer t
+        flag_mpsc۰consumer t
     }}}.
   Proof.
     iIntros "%Φ ((:inv =1) & (:consumer =2)) HΦ". simp.
     iDestruct (metaｰagree with "Hmeta_1 Hmeta_2") as %->. iClear "Hmeta_1".
 
-    wp۰apply (base.mpsc_flag٠getｰspec with "[$]") as (b) "Hb".
+    wp۰apply (base.flag_mpsc٠getｰspec with "[$]") as (b) "Hb".
     destruct b; iSteps.
   Qed.
 
-  Lemma mpsc_flag٠setｰspec t P :
+  Lemma flag_mpsc٠setｰspec t P :
     {{{
-      mpsc_flag۰inv t P ∗
+      flag_mpsc۰inv t P ∗
       ▷ P
     }}}
-      mpsc_flag٠set t
+      flag_mpsc٠set t
     {{{
       RET ();
-      mpsc_flag۰resolved t
+      flag_mpsc۰resolved t
     }}}.
   Proof.
     iIntros "%Φ ((:inv) & HP) HΦ".
 
-    wp۰apply (base.mpsc_flag٠setｰspec _ _ P with "[$]").
+    wp۰apply (base.flag_mpsc٠setｰspec _ _ P with "[$]").
     iSteps.
   Qed.
-End mpsc_flag۰G.
+End flag_mpsc۰G.
 
-#[global] Opaque mpsc_flag۰inv.
-#[global] Opaque mpsc_flag۰consumer.
-#[global] Opaque mpsc_flag۰resolved.
+#[global] Opaque flag_mpsc۰inv.
+#[global] Opaque flag_mpsc۰consumer.
+#[global] Opaque flag_mpsc۰resolved.
