theories/zoo_std/flag_mpsc__code.v
@@ -3,14 +3,14 @@ Require Import zoo.language.typeclasses.
 Require Import zoo.language.notations.
 Require Import zoo.options.
 
-Definition mpsc_flag٠create : val :=
+Definition flag_mpsc٠create : val :=
   𝗳𝘂𝗻 ⎽ ->
     𝗿𝗲𝗳 false.
 
-Definition mpsc_flag٠get : val :=
+Definition flag_mpsc٠get : val :=
   𝗳𝘂𝗻 "1" ->
     !"1".
 
-Definition mpsc_flag٠set : val :=
+Definition flag_mpsc٠set : val :=
   𝗳𝘂𝗻 "t" ->
     "t" <- true.
