theories/zoo_std/flag_mpsc__opaque.v
@@ -1,0 +1,5 @@
+Require Import zoo_std.flag_mpsc__code.
+
+#[global] Opaque flag_mpsc٠create.
+#[global] Opaque flag_mpsc٠get.
+#[global] Opaque flag_mpsc٠set.
