theories/zoo_std/mpsc_flag__opaque.v
@@ -1,5 +1,0 @@
-Require Import zoo_std.mpsc_flag__code.
-
-#[global] Opaque mpsc_flag٠create.
-#[global] Opaque mpsc_flag٠get.
-#[global] Opaque mpsc_flag٠set.
